LambdaS5/caml/ljs/ljs_parser.mly
@@ -1,15 +1,48 @@
 %{
+open Ljs_syntax
 
-open Syntax
+let with_pos exp pos = match exp with
+  | Null _ -> Null pos
+  | Undefined _ -> Undefined pos
+  | String (_, str) -> String (pos, str)
+  | Num (_, num) -> Num (pos, num)
+  | True _ -> True pos
+  | False _ -> False pos
+  | Id (_, id) -> Id (pos, id)
+  | Object (_, attrs, props) -> Object (pos, attrs, props)
+  | GetAttr (_, pattr, obj, field) -> GetAttr (pos, pattr, obj, field)
+  | SetAttr (_, prop, obj, field, value) -> SetAttr (pos, prop, obj, field, value)
+  | GetObjAttr (_, oattr, obj) -> GetObjAttr (pos, oattr, obj)
+  | SetObjAttr (_, oattr, obj, v) -> SetObjAttr (pos, oattr, obj, v)
+  | GetField (_, left, right, args) -> GetField (pos, left, right, args)
+  | SetField (_, obj, field, value, args) -> SetField (pos, obj, field, value, args)
+  | DeleteField (_, obj, field) -> DeleteField (pos, obj, field)
+  | OwnFieldNames (_, obj) -> OwnFieldNames(pos, obj)
+  | SetBang (_, id, exp) -> SetBang (pos, id, exp)
+  | Op1 (_, op, exp) -> Op1 (pos, op, exp)
+  | Op2 (_, op, left, right) -> Op2 (pos, op, left, right)
+  | If (_, test, trueBlock, falseBlock) -> If (pos, test, trueBlock, falseBlock)
+  | App (_, func, args) -> App (pos, func, args)
+  | Seq (_, left, right) -> Seq (pos, left, right)
+  | Let (_, id, value, body) -> Let (pos, id, value, body)
+  | Rec (_, id, value, body) -> Rec (pos, id, value, body)
+  | Label (_, id, exp) -> Label (pos, id, exp)
+  | Break (_, id, exp) -> Break (pos, id, exp)
+  | TryCatch (_, tryBlock, catchBlock) -> TryCatch (pos, tryBlock, catchBlock)
+  | TryFinally (_, tryBlock, finallyBlock) -> TryFinally (pos, tryBlock, finallyBlock)
+  | Throw (_, value) -> Throw (pos, value)
+  | Lambda (_, ids, body) -> Lambda (pos, ids, body)
+  | Eval (_, exp, obj) -> Eval (pos, exp, obj)
+  | Hint (_, label, exp) -> Hint (pos, label, exp)
 
 %}
 
 %token <int> INT
 %token <float> NUM
-%token <char list> STRING
-%token <char list> HINT
+%token <string> STRING
+%token <string> HINT
 %token <bool> BOOL
-%token <char list> ID
+%token <string> ID
 %token UNDEFINED NULL FUNC LET DELETE LBRACE RBRACE LPAREN RPAREN LBRACK
   RBRACK EQUALS COMMA DEREF REF COLON COLONEQ PRIM IF ELSE SEMI
   LABEL BREAK TRY CATCH FINALLY THROW EQEQEQUALS TYPEOF
@@ -26,41 +59,42 @@ open Syntax
 %left ELSE
 %left LPAREN
 
-%type <Syntax.expression> prog
-%type <Syntax.expression -> Syntax.expression> env
+%type <Ljs_syntax.exp> prog
+%type <Ljs_syntax.exp -> Ljs_syntax.exp> env
 
 %start prog
 %start env
 
+
 %%
 
 const :
- | NUM { Number $1 }
- | INT {  Number (float_of_int $1) }
- | STRING { String $1 }
- | UNDEFINED { Undefined  }
- | NULL { Null }
- | BOOL { if $1
-          then True
-          else False }
+ | NUM { Num (Pos.real (Parsing.rhs_start_pos 1, Parsing.rhs_end_pos 1), $1) }
+ | INT {  Num (Pos.real (Parsing.rhs_start_pos 1, Parsing.rhs_end_pos 1), (float_of_int $1)) }
+ | STRING {  String (Pos.real (Parsing.rhs_start_pos 1, Parsing.rhs_end_pos 1), $1) }
+ | UNDEFINED { Undefined (Pos.real (Parsing.rhs_start_pos 1, Parsing.rhs_end_pos 1)) }
+ | NULL { Null (Pos.real (Parsing.rhs_start_pos 1, Parsing.rhs_end_pos 1)) }
+ | BOOL { if $1 
+          then True (Pos.real (Parsing.rhs_start_pos 1, Parsing.rhs_end_pos 1)) 
+          else False (Pos.real (Parsing.rhs_start_pos 1, Parsing.rhs_end_pos 1)) }
 
 more_oattrs :
  | COMMA oattrsv { $2 }
- | COMMA { default_object_attributes }
- | { default_object_attributes }
+ | COMMA { d_attrs }
+ | { d_attrs }
 
 oattrsv :
- | PRIMVAL COLON exp more_oattrs { match $4 with ObjectAttributes (p, c, p', k, e) -> ObjectAttributes (Some $3, c, p', k, e) }
- | EXTENSIBLE COLON BOOL more_oattrs { match $4 with ObjectAttributes (p, c, p', k, e) -> ObjectAttributes (p, c, p', k, $3) }
- | PROTO COLON exp more_oattrs { match $4 with ObjectAttributes (p, c, p', k, e) -> ObjectAttributes (p, c, Some $3, k, e) }
- | CODE COLON exp more_oattrs { match $4 with ObjectAttributes (p, c, p', k, e) -> ObjectAttributes (p, Some $3, p', k, e) }
- | CLASS COLON STRING more_oattrs { match $4 with ObjectAttributes (p, c, p', k, e) -> ObjectAttributes (p, c, p', $3, e) }
+ | PRIMVAL COLON exp more_oattrs { { $4 with primval = Some $3 } }
+ | EXTENSIBLE COLON BOOL more_oattrs { { $4 with extensible = $3 } }
+ | PROTO COLON exp more_oattrs { { $4 with proto = Some $3 } }
+ | CODE COLON exp more_oattrs { {$4 with code = Some $3 } }
+ | CLASS COLON STRING more_oattrs { { $4 with klass = $3 } }
 
 oattr_name :
  | PRIMVAL { Primval }
  | PROTO { Proto }
  | CODE { Code }
- | CLASS { Class }
+ | CLASS { Klass }
  | EXTENSIBLE { Extensible }
 
 attr_name :
@@ -73,15 +107,15 @@ attr_name :
 
 prop_attrs :
  | VALUE exp COMMA WRITABLE BOOL
-     { DataProperty (Data ($2, $5), false, false) }
+     { Data ({ value = $2; writable = $5 }, false, false) }
  | VALUE exp COMMA WRITABLE BOOL COMMA CONFIG BOOL
-     { DataProperty (Data ($2, $5), false, $8) }
+     { Data ({ value = $2; writable = $5 }, false, $8) }
  | VALUE exp COMMA WRITABLE BOOL COMMA CONFIG BOOL COMMA ENUM BOOL
-     { DataProperty (Data ($2, $5), $11, $8) }
+     { Data ({ value = $2; writable = $5 }, $11, $8) }
  | VALUE exp COMMA WRITABLE BOOL COMMA ENUM BOOL COMMA CONFIG BOOL
-     { DataProperty (Data ($2, $5), $8, $11) }
+     { Data ({ value = $2; writable = $5 }, $8, $11) }
  | GETTER exp COMMA SETTER exp
-     { AccessorProperty (Accessor ($2, $5), false, true) }
+     { Accessor ({ getter = $2; setter = $5 }, false, true) }
 
 prop :
  | STRING COLON LBRACE prop_attrs RBRACE { ($1, $4) }
@@ -103,113 +137,136 @@ ids :
  | ID COMMA ids { $1 :: $3 }
 
 func :
- | FUNC LPAREN ids RPAREN braced_seq_exp { Lambda ($3, $5) }
+ | FUNC LPAREN ids RPAREN braced_seq_exp
+   { Lambda (Pos.real (Parsing.rhs_start_pos 1, Parsing.rhs_end_pos 5), $3, $5) }
 
 atom :
  | const { $1 }
- | ID { Id $1 }
- | LBRACE LBRACK oattrsv RBRACK props RBRACE { ObjectDecl ($3, $5)}
- | LBRACE LBRACK RBRACK props RBRACE { ObjectDecl (default_object_attributes, $4 )}
- | braced_seq_exp { $1 }
+ | ID { Id (Pos.real (Parsing.rhs_start_pos 1, Parsing.rhs_end_pos 1), $1) }
+ | LBRACE LBRACK oattrsv RBRACK props RBRACE 
+   { Object (Pos.real (Parsing.rhs_start_pos 1, Parsing.rhs_end_pos 6), $3, $5 )}
+ | LBRACE LBRACK RBRACK props RBRACE 
+   { Object (Pos.real (Parsing.rhs_start_pos 1, Parsing.rhs_end_pos 6), d_attrs, $4 )}
+ | braced_seq_exp
+   { $1 }
  | LPAREN unbraced_seq_exp RPAREN { $2 }
  | func { $1 }
- | TYPEOF atom { Op1 (CoqUtils.explode "typeof", $2) }
+ | TYPEOF atom
+     { Op1 (Pos.real (Parsing.rhs_start_pos 1, Parsing.rhs_end_pos 2), "typeof", $2) }
      
 exp :
  | atom { $1 }
  | exp LPAREN exps RPAREN 
-   { App ($1, $3) }
+   { App (Pos.real (Parsing.rhs_start_pos 1, Parsing.rhs_end_pos 4), $1, $3) }
  | GETFIELDS LPAREN exp RPAREN
-   { OwnFieldNames $3 }
+   { OwnFieldNames (Pos.real (Parsing.rhs_start_pos 1, Parsing.rhs_end_pos 4), $3) }
  | EVAL LPAREN exp COMMA exp RPAREN
-     { Eval ($3, $5) }
+     { Eval (Pos.real (Parsing.rhs_start_pos 1, Parsing.rhs_end_pos 4), $3, $5) }
  | PRIM LPAREN STRING COMMA unbraced_seq_exp COMMA unbraced_seq_exp RPAREN
-   { Op2 ($3, $5, $7) }
+   { Op2 (Pos.real (Parsing.rhs_start_pos 1, Parsing.rhs_end_pos 8), $3, $5, $7) }
  | PRIM LPAREN STRING COMMA unbraced_seq_exp RPAREN
-   { Op1 ($3, $5) }
+   { Op1 (Pos.real (Parsing.rhs_start_pos 1, Parsing.rhs_end_pos 6), $3, $5) }
  | ID COLONEQ exp
-   { SetBang ($1, $3) }
+   { SetBang (Pos.real (Parsing.rhs_start_pos 1, Parsing.rhs_end_pos 3), $1, $3) }
  | exp EQEQEQUALS exp
-     { Op2 (CoqUtils.explode "stx=", $1, $3) }
+     { Op2 (Pos.real (Parsing.rhs_start_pos 1, Parsing.rhs_end_pos 3), "stx=", $1, $3) }
  | exp BANGEQEQUALS exp
-     { If (Op2 (CoqUtils.explode "stx=", $1, $3), False, True) }
+     { let p = Pos.real (Parsing.rhs_start_pos 1, Parsing.rhs_end_pos 3) in
+         If (p, Op2 (p, "stx=", $1, $3),
+             False p, True p) }
  | exp LBRACK unbraced_seq_exp EQUALS unbraced_seq_exp RBRACK
-   { Let (CoqUtils.explode "$newVal", $5,
-	     SetField ($1, $3, 
-		       Id (CoqUtils.explode "$newVal"), 
-		       ObjectDecl (default_object_attributes,
-            [(CoqUtils.explode "0", DataProperty (Data (Id (CoqUtils.explode "$newVal"), true),
+   { let p = Pos.real (Parsing.rhs_start_pos 1, Parsing.rhs_end_pos 6) in
+       Let (p, "$newVal", $5,
+	     SetField (p, $1, $3, 
+		       Id (p, "$newVal"), 
+		       Object (p, d_attrs,
+            [("0", Data ({ value = Id (p, "$newVal");
+                          writable = true },
               true, true))])))
     }
  | exp LBRACK unbraced_seq_exp EQUALS unbraced_seq_exp COMMA unbraced_seq_exp RBRACK
-   { SetField ($1, $3, $5, $7) }
+   { SetField (Pos.real (Parsing.rhs_start_pos 1, Parsing.rhs_end_pos 8), $1, $3, $5, $7) }
  | exp LBRACK unbraced_seq_exp RBRACK
-   { GetField ($1,  $3,
-		       ObjectDecl (default_object_attributes, [])) }
+   { let p = Pos.real (Parsing.rhs_start_pos 1, Parsing.rhs_end_pos 4) in
+     GetField (p, $1,  $3,
+		       Object (p, d_attrs,
+            [])) }
  | exp LBRACK unbraced_seq_exp COMMA unbraced_seq_exp RBRACK
-   { GetField ($1, $3, $5) }
+   { GetField (Pos.real (Parsing.rhs_start_pos 1, Parsing.rhs_end_pos 6), $1, $3, $5) }
  | exp LBRACK DELETE unbraced_seq_exp RBRACK
-     { DeleteField ($1, $4) }
+     { DeleteField (Pos.real (Parsing.rhs_start_pos 1, Parsing.rhs_end_pos 5), $1, $4) }
  | exp LBRACK unbraced_seq_exp LT attr_name GT RBRACK
-     { GetAttr ($5, $1, $3) }
+     { GetAttr (Pos.real (Parsing.rhs_start_pos 1, Parsing.rhs_end_pos 7), $5, $1, $3) }
  | exp LBRACK unbraced_seq_exp LT attr_name GT EQUALS unbraced_seq_exp RBRACK
-     { SetAttr ($5, $1, $3, $8) }
+     { SetAttr (Pos.real (Parsing.rhs_start_pos 1, Parsing.rhs_end_pos 9), $5, $1, $3, $8) }
  | exp LBRACK LT oattr_name GT RBRACK
-     { GetObjAttr($4, $1) }
+     { GetObjAttr(Pos.real (Parsing.rhs_start_pos 1, Parsing.rhs_end_pos 6),
+                  $4, $1) }
  | exp LBRACK LT oattr_name GT EQUALS unbraced_seq_exp RBRACK
-     { SetObjAttr($4, $1, $7) }
- | exp AMPAMP exp { If ($1, $3, False) }
+     { SetObjAttr(Pos.real (Parsing.rhs_start_pos 1, Parsing.rhs_end_pos 8),
+                  $4, $1, $7) }
+ | exp AMPAMP exp
+     { If (Pos.real (Parsing.rhs_start_pos 1, Parsing.rhs_end_pos 3), $1, 
+            $3, False (Pos.real (Parsing.rhs_start_pos 1, Parsing.rhs_end_pos 3))) }
  | exp PIPEPIPE exp
-     { Let (CoqUtils.explode "%or", $1, If (Id (CoqUtils.explode "%or"), Id (CoqUtils.explode "%or"), $3)) }
+     { let p = Pos.real (Parsing.rhs_start_pos 1, Parsing.rhs_end_pos 3) in
+         Let (p, "%or", $1,
+               If (p, Id (p, "%or"), Id (p, "%or"), $3)) }
 
 
 cexp :
  | exp { $1 }
  | ifexp { $1 }
  | LPAREN HINT cexp RPAREN
-     { Hint ($2, $3) }
+     { Hint (Pos.real (Parsing.rhs_start_pos 1, Parsing.rhs_end_pos 4), $2, $3) }
  | LABEL ID COLON braced_seq_exp
-     { Label ($2, $4) } 
+     { Label (Pos.real (Parsing.rhs_start_pos 1, Parsing.rhs_end_pos 4), $2, $4) } 
  | BREAK ID cexp
-   { Break ($2, $3) }
+   { Break (Pos.real (Parsing.rhs_start_pos 1, Parsing.rhs_end_pos 3), $2, $3) }
  | THROW cexp
-   { Throw ($2) }
+   { Throw (Pos.real (Parsing.rhs_start_pos 1, Parsing.rhs_end_pos 2), $2) }
  | TRY braced_seq_exp CATCH braced_seq_exp
-   { TryCatch ($2, $4) }
+   { TryCatch (Pos.real (Parsing.rhs_start_pos 1, Parsing.rhs_end_pos 4), $2, $4) }
  | TRY braced_seq_exp FINALLY braced_seq_exp
-   { TryFinally ($2, $4) }
+   { TryFinally (Pos.real (Parsing.rhs_start_pos 1, Parsing.rhs_end_pos 4), $2, $4) }
 
 ifexp :
  | IF LPAREN unbraced_seq_exp RPAREN braced_seq_exp ELSE ifexp
-     { If ($3, $5, $7) }
+     { If (Pos.real (Parsing.rhs_start_pos 1, Parsing.rhs_end_pos 7), $3, $5, $7) }
  | IF LPAREN unbraced_seq_exp RPAREN braced_seq_exp ELSE braced_seq_exp
-     { If ($3, $5, $7) }
+     { If (Pos.real (Parsing.rhs_start_pos 1, Parsing.rhs_end_pos 7), $3, $5, $7) }
  | IF LPAREN unbraced_seq_exp RPAREN braced_seq_exp
-     { If ($3, $5, Undefined) }
+     { If (Pos.real (Parsing.rhs_start_pos 1, Parsing.rhs_end_pos 5), $3, $5, 
+	    Undefined (Pos.real (Parsing.rhs_start_pos 1, Parsing.rhs_end_pos 5))) }
 
 braced_seq_exp :
- | LBRACE unbraced_seq_exp RBRACE { $2 }
+ | LBRACE unbraced_seq_exp RBRACE { with_pos $2 (Pos.real (Parsing.rhs_start_pos 1, Parsing.rhs_end_pos 3)) }
 
 unbraced_seq_exp :
- | unbraced_seq_item SEMI unbraced_seq_exp { Seq ($1, $3) }
+ | unbraced_seq_item SEMI unbraced_seq_exp { Seq (Pos.real (Parsing.rhs_start_pos 1, Parsing.rhs_end_pos 3), $1, $3) }
  | unbraced_seq_item { $1 }
 
 unbraced_seq_item :
  | cexp { $1 }
  | LET LPAREN ID EQUALS unbraced_seq_exp RPAREN unbraced_seq_item
-   { Let ($3, $5, $7) }
+   { Let (Pos.real (Parsing.rhs_start_pos 1, Parsing.rhs_end_pos 7), $3, $5, $7) }
  | REC LPAREN ID EQUALS func RPAREN unbraced_seq_item
-   { Rec ($3, $5, $7) }
+   { Rec (Pos.real (Parsing.rhs_start_pos 1, Parsing.rhs_end_pos 7), $3, $5, $7) }
 
 env :
  | EOF
      { fun x -> x }
  | LET LBRACK ID RBRACK EQUALS unbraced_seq_exp env
-     { fun x -> 
-           Let ($3, $6, $7 x) }
+     { let p = Pos.real (Parsing.rhs_start_pos 1, Parsing.rhs_end_pos 7) in
+         fun x -> 
+           Let (p, $3, $6, $7 x) }
  | REC LBRACK ID RBRACK EQUALS unbraced_seq_exp env
-     { fun x -> Rec ($3, $6, $7 x) }
- | braced_seq_exp env { fun x -> Seq ($1, $2 x) }
+     { let p = Pos.real (Parsing.rhs_start_pos 1, Parsing.rhs_end_pos 7) in
+         fun x -> 
+           Rec (p, $3, $6, $7 x) }
+ | braced_seq_exp env
+     { let p = Pos.real (Parsing.rhs_start_pos 1, Parsing.rhs_end_pos 2) in
+         fun x -> Seq (p, $1, $2 x) }
 
 prog :
  | unbraced_seq_exp EOF { $1 }
