LambdaS5/coq/Syntax.v
@@ -13,66 +13,66 @@ Definition id : Type := string.
 
 Definition number : Type := Fappli_IEEE_bits.binary64.
 
-Inductive object_attribute_name : Type :=
-| Proto
-| Class
-| Extensible
-| Primval
-| Code
+Inductive oattr : Type := (* object attribute name *)
+| oattr_proto
+| oattr_class
+| oattr_extensible
+| oattr_primval
+| oattr_code
 .
 
-Inductive property_attribute_name : Type :=
-| Value
-| Getter
-| Setter
-| Config
-| Writable
-| Enum
+Inductive pattr : Type := (* property attribute name *)
+| pattr_value
+| pattr_getter
+| pattr_setter
+| pattr_config
+| pattr_writable
+| pattr_enum
 .
 
 
-Inductive expression : Type :=
-| Null
-| Undefined
-| String : string -> expression
-| Number : number -> expression
-| True
-| False
-| Id : id -> expression
-| ObjectDecl : object_attributes -> list (string * property) -> expression
-| GetAttr : property_attribute_name -> expression -> expression -> expression (* property -> object -> field_name -> expression *)
-| SetAttr : property_attribute_name -> expression -> expression -> expression -> expression (* property -> object -> field_name -> new_value -> expression *)
-| GetObjAttr : object_attribute_name -> expression -> expression
-| SetObjAttr : object_attribute_name -> expression -> expression -> expression
-| GetField : expression -> expression -> expression -> expression (* left -> right -> args_object -> expression *)
-| SetField : expression -> expression -> expression -> expression -> expression (* object -> field -> new_val -> args -> expression *)
-| DeleteField : expression -> expression -> expression (* object -> field -> expression *)
-| OwnFieldNames : expression -> expression
-| SetBang : id -> expression -> expression
-| Op1 : string -> expression -> expression
-| Op2 : string -> expression -> expression -> expression
-| If : expression -> expression -> expression -> expression
-| App : expression -> list expression -> expression
-| Seq : expression -> expression -> expression
-| Let : id -> expression -> expression -> expression
-| Rec : id -> expression -> expression -> expression (* Value bound must be lambda *)
-| Label : id -> expression -> expression
-| Break : id -> expression -> expression
-| TryCatch : expression -> expression -> expression (* Catch block must be a lambda *)
-| TryFinally : expression -> expression -> expression
-| Throw : expression -> expression
-| Lambda : list id -> expression -> expression
-| Eval : expression -> expression -> expression (* string -> env_object -> expression *)
-| Hint : string -> expression -> expression
+Inductive expr : Type :=
+| expr_null
+| expr_undefined
+| expr_string : string -> expr
+| expr_number : number -> expr
+| expr_true
+| expr_false
+| expr_id : id -> expr
+| expr_object : objattrs -> list (string * property) -> expr
+| expr_get_attr : pattr -> expr -> expr -> expr (* property -> object -> field_name -> expr *)
+| expr_set_attr : pattr -> expr -> expr -> expr -> expr (* property -> object -> field_name -> new_value -> expr *)
+| expr_get_obj_attr : oattr -> expr -> expr
+| expr_set_obj_attr : oattr -> expr -> expr -> expr
+| expr_get_field : expr -> expr -> expr -> expr (* left -> right -> args_object -> expr *)
+| expr_set_field : expr -> expr -> expr -> expr -> expr (* object -> field -> new_val -> args -> expr *)
+| expr_delete_field : expr -> expr -> expr (* object -> field -> expr *)
+| expr_own_field_names : expr -> expr
+| expr_set_bang : id -> expr -> expr
+| expr_op1 : string -> expr -> expr
+| expr_op2 : string -> expr -> expr -> expr
+| expr_if : expr -> expr -> expr -> expr
+| expr_app : expr -> list expr -> expr
+| expr_seq : expr -> expr -> expr
+| expr_let : id -> expr -> expr -> expr
+| expr_recc : id -> expr -> expr -> expr (* Value bound must be lambda *)
+| expr_label : id -> expr -> expr
+| expr_break : id -> expr -> expr
+| expr_try_catch : expr -> expr -> expr (* Catch block must be a lambda *)
+| expr_try_finally : expr -> expr -> expr
+| expr_throw : expr -> expr
+| expr_lambda : list id -> expr -> expr
+| expr_eval : expr -> expr -> expr (* string -> env_object -> expr *)
+| expr_hint : string -> expr -> expr
 with data : Type :=
-| Data : expression -> bool -> data (* expression -> writable -> data *)
+| data_intro : expr -> bool -> data (* expr -> writable -> data *)
 with accessor : Type :=
-| Accessor : expression -> expression -> accessor (* getter -> setter -> accessor *)
+| accessor_intro : expr -> expr -> accessor (* getter -> setter -> accessor *)
 with property : Type := 
-| DataProperty : data -> bool -> bool -> property (* value -> enumerable -> configurable *)
-| AccessorProperty : accessor -> bool -> bool -> property
-with object_attributes : Type :=
-| ObjectAttributes: option expression -> option expression -> option expression -> string -> bool -> object_attributes (* primval -> code -> prototype -> class -> extensible -> object_attributes *)
+| property_data : data -> bool -> bool -> property (* value -> enumerable -> configurable *)
+| property_accessor : accessor -> bool -> bool -> property
+with objattrs : Type :=
+| objattrs_intro : option expr -> option expr -> option expr -> string -> bool -> objattrs (* primval -> code -> prototype -> class -> extensible -> objattrs *)
 .
 
-Definition default_object_attributes := ObjectAttributes None None None "Object" true.
+Definition default_objattrs := objattrs_intro None None None "Object" true.
